SlowTest/DiffLogic-Test/seq_Boogie.bpl
@@ -14,56 +14,56 @@ procedure S0'() returns (a: [int]bool)
     assert (forall j:int :: j == 0 ==> a[j]); // quantifier tactic?
 }
 
-procedure S1(len: int) returns (a: [int]bool)
-  requires 0 < len;
-  ensures (forall j: int :: 0 <= j && j < len ==> a[j]);
-{
-    var i: int;
-    i := 0;
-    a[0] := true;
-    while ( i < len )
-        invariant 0 <= i && i <= len;
-        invariant (forall j: int :: {a[j]} 0 <= j && j < i ==> a[j]);
-    {
-        a[i] := true;
-        // assume a[i]; // not work
-        // assert (forall j: int :: 0 <= j && j < i ==> a[j]);
-        // assume (forall j: int :: {a[j]} i == j ==> a[j]);
+// procedure S1(len: int) returns (a: [int]bool)
+//   requires 0 < len;
+//   ensures (forall j: int :: 0 <= j && j < len ==> a[j]);
+// {
+//     var i: int;
+//     i := 0;
+//     a[0] := true;
+//     while ( i < len )
+//         invariant 0 <= i && i <= len;
+//         invariant (forall j: int :: {a[j]} 0 <= j && j < i ==> a[j]);
+//     {
+//         a[i] := true;
+//         // assume a[i]; // not work
+//         // assert (forall j: int :: 0 <= j && j < i ==> a[j]);
+//         // assume (forall j: int :: {a[j]} i == j ==> a[j]);
 
-        // assert (forall j: int :: i == j ==> 0 <= j && j < i + 1 ==> a[j]);
-        // assert (forall j: int :: i != j ==> 0 <= j && j < i + 1 ==> a[j]);
+//         // assert (forall j: int :: i == j ==> 0 <= j && j < i + 1 ==> a[j]);
+//         // assert (forall j: int :: i != j ==> 0 <= j && j < i + 1 ==> a[j]);
 
-        // assert (0 <= i && i < i + 1 ==> a[i]);
+//         // assert (0 <= i && i < i + 1 ==> a[i]);
 
-        i := i + 1;
-    }
-}
+//         i := i + 1;
+//     }
+// }
 
-procedure S2(in: [int]int, len: int) returns (out: [int]int)
-//   requires in[0] == 0 && (forall i: int :: 0 <= i && i < len - 1 ==> in[i + 1] == in[i] + 1); // works
-//   requires in[0] == 0 && (forall i: int :: 0 <= i ==> in[i] == 1); // works
-  requires in[0] == 0 && (forall i: int :: {in[i] + 1} 0 <= i ==> in[i + 1] == in[i] + 1); // need trigger to work
-  requires 0 < len;
-  ensures (forall j: int :: 0 <= j && j < len ==> out[j] == in[j]);
-{
-    var i : int;
+// procedure S2(in: [int]int, len: int) returns (out: [int]int)
+// //   requires in[0] == 0 && (forall i: int :: 0 <= i && i < len - 1 ==> in[i + 1] == in[i] + 1); // works
+// //   requires in[0] == 0 && (forall i: int :: 0 <= i ==> in[i] == 1); // works
+//   requires in[0] == 0 && (forall i: int :: {in[i] + 1} 0 <= i ==> in[i + 1] == in[i] + 1); // need trigger to work
+//   requires 0 < len;
+//   ensures (forall j: int :: 0 <= j && j < len ==> out[j] == in[j]);
+// {
+//     var i : int;
 
-    i := 0;
-    out[i] := 0;
-    while (i < len)
-      invariant 0 <= i && i <= len;
-      invariant out[0] == 0 && (forall j: int :: 0 <= j && j < i ==> out[j] == in[j]);
-    {
-        out[i] := in[i];
-        // assume (forall j: int :: i == j ==> out[j] == in[j]);
-        i := i + 1;
-    }
+//     i := 0;
+//     out[i] := 0;
+//     while (i < len)
+//       invariant 0 <= i && i <= len;
+//       invariant out[0] == 0 && (forall j: int :: 0 <= j && j < i ==> out[j] == in[j]);
+//     {
+//         out[i] := in[i];
+//         // assume (forall j: int :: i == j ==> out[j] == in[j]);
+//         i := i + 1;
+//     }
 
-    i := 0;
-    while (i < len)
-      invariant 0 <= i && i <= len;
-      invariant (forall j: int :: 0 <= j && j < i ==> out[j] == in[j]);
-    {
-        i := i + 1;
-    }
-}
+//     i := 0;
+//     while (i < len)
+//       invariant 0 <= i && i <= len;
+//       invariant (forall j: int :: 0 <= j && j < i ==> out[j] == in[j]);
+//     {
+//         i := i + 1;
+//     }
+// }
