SlowTest/DiffLogic-Test/test_Dafny.dfy
@@ -1,6 +1,8 @@
 method myAdd(a: int, b: int)
     { assert a == 10 && b == 11 ==> a + b == 21; }
 
+method simple ()
+    {assert 0 < 2; }
 // function method Add(a: int, b: int): int { a + b }
 // function method Sub(a: int, b: int): int { a - b }
 
